theories/Compl.v
@@ -199,18 +199,18 @@ Module Type COMPL_F(Import Conf : DETECT_CONF)(Import Params : DETECT_PARAMS(Con
         apply SRPC_Finger.
     Qed.
 
-    Lemma SRPC_sane_Echo : SRPC_sane Free (pq [] Echo []).
+    Lemma SRPC_sane_Echo : SRPC_sane Free (serv [] Echo []).
       constructor; intros; doubt.
       eauto using SRPC_Echo with LTS.
     Qed.
 
-    Lemma SRPC_sane_Finger : forall n, SRPC_sane (Lock (nat_Name (S (S n))) (nat_Name n)) (pq [] (MoverFinger (nat_Name (S n))) []).
+    Lemma SRPC_sane_Finger : forall n, SRPC_sane (Lock (nat_Name (S (S n))) (nat_Name n)) (serv [] (MoverFinger (nat_Name (S n))) []).
       intros.
       constructor; intros; doubt.
       eauto using SRPC_Finger with LTS.
     Qed.
 
-    Lemma SRPC_sane_Nail : SRPC_sane (Work (nat_Name 2)) (pq [] MoverNail []).
+    Lemma SRPC_sane_Nail : SRPC_sane (Work (nat_Name 2)) (serv [] MoverNail []).
       constructor; intros; doubt.
       eauto using SRPC_Nail with LTS.
     Qed.
@@ -218,7 +218,7 @@ Module Type COMPL_F(Import Conf : DETECT_CONF)(Import Params : DETECT_PARAMS(Con
     Example t_Net : {N : PNet | Mover N (nat_Name 1) /\ net_sane N}.
     pose (N := NetMod.init
                  (
-                   fun n => (pq [] (
+                   fun n => (serv [] (
                                  match Name_nat n with
                                  | 0 => Echo
                                  | S 0 => MoverNail
@@ -1034,7 +1034,7 @@ Module Type COMPL_F(Import Conf : DETECT_CONF)(Import Params : DETECT_PARAMS(Con
 
 
   Lemma SRPC_pq_no_immediate_relock [n0 n1 S0 S1 a] :
-    AnySRPC_pq S0 ->
+    AnySRPC_serv S0 ->
     (S0 =(a)=> S1) ->
     pq_lock [n0] S0 ->
     pq_lock [n1] S1 ->
@@ -1090,7 +1090,7 @@ Module Type COMPL_F(Import Conf : DETECT_CONF)(Import Params : DETECT_PARAMS(Con
 
 
   (* Lemma SRPC_net_no_immediate_relock [n m0 m1 N0 N1 a] : *)
-  (*   (forall n, AnySRPC_pq (NetMod.get n N0)) -> *)
+  (*   (forall n, AnySRPC_serv (NetMod.get n N0)) -> *)
   (*   (N0 =(a)=> N1) -> *)
   (*   net_lock_on N0 n m0 -> *)
   (*   net_lock_on N1 n m1 -> *)
@@ -1133,7 +1133,7 @@ Module Type COMPL_F(Import Conf : DETECT_CONF)(Import Params : DETECT_PARAMS(Con
 
 
   Lemma SRPC_M_net_no_immediate_relock [n m0 m1 N0 N1 a] :
-    (forall n, AnySRPC_pq (NetMod.get n '' N0)) ->
+    (forall n, AnySRPC_serv (NetMod.get n '' N0)) ->
     (N0 =(a)=> N1) ->
     net_lock_on '' N0 n m0 ->
     net_lock_on '' N1 n m1 ->
@@ -1162,7 +1162,7 @@ Module Type COMPL_F(Import Conf : DETECT_CONF)(Import Params : DETECT_PARAMS(Con
   (*   destruct (NetMod.get n0 N0) as [I0 P0 O0] eqn:?. *)
   (*   destruct (NetMod.get n0 N1) as [I1 P1 O1] eqn:?. *)
 
-  (*   assert (exists c, SRPC_pq (Lock c n1) (NetMod.get n0 N1)). *)
+  (*   assert (exists c, SRPC_serv (Lock c n1) (NetMod.get n0 N1)). *)
   (*   { *)
   (*     apply lock_singleton in H1. 2: attac. *)
   (*     unfold net_lock in *. *)
@@ -1176,10 +1176,10 @@ Module Type COMPL_F(Import Conf : DETECT_CONF)(Import Params : DETECT_PARAMS(Con
   (*     unfold net_lock in *. *)
   (*     rewrite `(NetMod.get n0 N1 = _) in *. *)
   (*     compat_hsimpl in *. *)
-  (*     consider (pq_lock [n1] (pq _ _ _)). *)
+  (*     consider (pq_lock [n1] (serv _ _ _)). *)
   (*     destruct P1; doubt. *)
   (*     eattac 3. *)
-  (*     consider (exists c', SRPC_pq (Lock c' m) (NetMod.get n0 N1)) by eauto with LTS. *)
+  (*     consider (exists c', SRPC_serv (Lock c' m) (NetMod.get n0 N1)) by eauto with LTS. *)
   (*     consider (Lock c' m = Lock c n1) by eauto with LTS. *)
   (*     bs (List.In (n1, R, v) I1). *)
   (*   } *)
@@ -1401,7 +1401,7 @@ Module Type COMPL_F(Import Conf : DETECT_CONF)(Import Params : DETECT_PARAMS(Con
 
 
   Lemma SRPC_pq_client_dec [n S] :
-    AnySRPC_pq S ->
+    AnySRPC_serv S ->
     pq_client n S \/ ~ pq_client n S.
 
   Proof.
@@ -2085,7 +2085,7 @@ Module Type COMPL_F(Import Conf : DETECT_CONF)(Import Params : DETECT_PARAMS(Con
     apply Forall_forall.
     intros.
     destruct x; auto.
-    destruct (deinstr (mq MQ0 M0 (pq I0 P0 O0))) as [I' P' O'] eqn:?.
+    destruct (deinstr (mq MQ0 M0 (serv I0 P0 O0))) as [I' P' O'] eqn:?.
     absurd (List.In (n0, v) O').
     - intros ?.
       unfold deinstr in *.
@@ -2097,7 +2097,7 @@ Module Type COMPL_F(Import Conf : DETECT_CONF)(Import Params : DETECT_PARAMS(Con
       clear - H0 H1.
       induction l; attac.
       destruct a; attac.
-    - assert (deinstr (mq l m p) = pq I' P' O') by attac.
+    - assert (deinstr (mq l m p) = serv I' P' O') by attac.
       eapply (deinstr_In_send `(List.In _ l)). attac.
   Qed.
 
@@ -2729,7 +2729,7 @@ Module Type COMPL_F(Import Conf : DETECT_CONF)(Import Params : DETECT_PARAMS(Con
 
   (* (* TODO TO LOCKS *) *)
   (* Lemma lock_no_dep_refute [N] [n0 n1 n2] : *)
-  (*   (forall n, AnySRPC_pq (NetMod.get n N)) -> *)
+  (*   (forall n, AnySRPC_serv (NetMod.get n N)) -> *)
   (*   n1 <> n2 -> *)
   (*   net_lock_on N n0 n1 -> *)
   (*   ~ dep_on N n1 n2 -> *)
@@ -2749,7 +2749,7 @@ Module Type COMPL_F(Import Conf : DETECT_CONF)(Import Params : DETECT_PARAMS(Con
 
 
   (* Lemma lock_no_dep_refute' [N] [n0 n1 n2] : *)
-  (*   (forall n, AnySRPC_pq (NetMod.get n N)) -> *)
+  (*   (forall n, AnySRPC_serv (NetMod.get n N)) -> *)
   (*   net_lock_on N n0 n1 -> *)
   (*   ~ dep_on N n0 n2 -> *)
   (*   ~ dep_on N n1 n2. *)
@@ -2804,7 +2804,7 @@ Module Type COMPL_F(Import Conf : DETECT_CONF)(Import Params : DETECT_PARAMS(Con
       ltac1:(autorewrite with LTS in * ).
       rewrite `(NetMod.get n MN0 = _) in *.
       destruct S.
-      enough (deinstr (mq MQ M (pq l p l0)) = pq &I P []) by eauto using deinstr_In_recv with LTS.
+      enough (deinstr (mq MQ M (serv l p l0)) = serv &I P []) by eauto using deinstr_In_recv with LTS.
       unfold deinstr; auto.
     }
 
@@ -2819,8 +2819,8 @@ Module Type COMPL_F(Import Conf : DETECT_CONF)(Import Params : DETECT_PARAMS(Con
         subst.
         unfold net_deinstr in *. simpl in *.
         ltac1:(autorewrite with LTS in * ).
-        enough (exists c0, SRPC_pq (Lock c0 n0) (pq I0 P0 O0)) by attac.
-        rewrite <- `(_ = pq I0 P0 O0).
+        enough (exists c0, SRPC_serv (Lock c0 n0) (serv I0 P0 O0)) by attac.
+        rewrite <- `(_ = serv I0 P0 O0).
 
         replace (deinstr (NetMod.get n MN0)) with (NetMod.get n '' MN0) by (unfold net_deinstr, deinstr; attac).
 
@@ -2843,8 +2843,8 @@ Module Type COMPL_F(Import Conf : DETECT_CONF)(Import Params : DETECT_PARAMS(Con
       eapply lock_SRPC_Lock.
       2: eattac.
 
-      enough (NetMod.get n '' MN0 = pq (&I ++ MQ_r MQ) P (MQ_s MQ ++ &O))
-        by (enough (AnySRPC_pq (pq (&I ++ MQ_r MQ) P (MQ_s MQ ++ &O))); eauto with LTS).
+      enough (NetMod.get n '' MN0 = serv (&I ++ MQ_r MQ) P (MQ_s MQ ++ &O))
+        by (enough (AnySRPC_serv (serv (&I ++ MQ_r MQ) P (MQ_s MQ ++ &O))); eauto with LTS).
 
       unfold net_deinstr, deinstr in *.
       ltac1:(autorewrite with LTS in * ).
@@ -3548,7 +3548,7 @@ Module Type COMPL_F(Import Conf : DETECT_CONF)(Import Params : DETECT_PARAMS(Con
   Proof with eattac.
     intros BSRPC Hd.
 
-    assert (forall n, AnySRPC_pq (NetMod.get n N)) as Hsrpc by eauto with LTS.
+    assert (forall n, AnySRPC_serv (NetMod.get n N)) as Hsrpc by eauto with LTS.
 
     consider (exists DS, List.In n0 DS /\ DeadSet DS N).
     hsimpl in *. (* TODO why? *)
@@ -4192,9 +4192,9 @@ Module Type COMPL_F(Import Conf : DETECT_CONF)(Import Params : DETECT_PARAMS(Con
           unfold deinstr in *.
           eattac.
         }
-        assert (NetMod.get n1 '' MN0 = pq &I P &O).
+        assert (NetMod.get n1 '' MN0 = serv &I P &O).
         {
-          rewrite <- `(_ = pq &I P &O).
+          rewrite <- `(_ = serv &I P &O).
           unfold net_deinstr, deinstr; hsimpl in *; hsimpl in *; attac.
         }
         eauto with LTS.
@@ -4232,9 +4232,9 @@ Module Type COMPL_F(Import Conf : DETECT_CONF)(Import Params : DETECT_PARAMS(Con
           unfold deinstr in *.
           eattac.
         }
-        assert (NetMod.get n1 '' MN0 = pq &I P &O).
+        assert (NetMod.get n1 '' MN0 = serv &I P &O).
         {
-          rewrite <- `(_ = pq &I P &O).
+          rewrite <- `(_ = serv &I P &O).
           unfold net_deinstr, deinstr; hsimpl in *; hsimpl in *; attac.
         }
         eauto with LTS.
@@ -4587,7 +4587,7 @@ Module Type COMPL_F(Import Conf : DETECT_CONF)(Import Params : DETECT_PARAMS(Con
                                       (mq
                                          ((l1 ++
                                              EvRecv (n', R) {| init := m; index := lock_id (next_state (state M)) |}
-                                             :: l2) ++ [TrSend (n, &t) v]) M (pq I0 P2 O1)) MN0)).
+                                             :: l2) ++ [TrSend (n, &t) v]) M (serv I0 P2 O1)) MN0)).
              2: eauto using net_lock_on_M_no_sends_in.
 
              intros Hx. clear - Hx.
@@ -4701,7 +4701,7 @@ Module Type COMPL_F(Import Conf : DETECT_CONF)(Import Params : DETECT_PARAMS(Con
 
       assert (dep_on '' MN1 n0 m0) by
         (destruct `(n0 = m0 \/ dep_on '' MN1 n0 m0); subst; eauto 4 using dep_reloop, dep_loop, dep_on_seq1 with LTS).
-      assert (forall n : Name, AnySRPC_pq (NetMod.get n '' MN1)) by re_have (eauto with LTS).
+      assert (forall n : Name, AnySRPC_serv (NetMod.get n '' MN1)) by re_have (eauto with LTS).
       assert (sends_probe (m0, R) (hot_of MN1 m1) (NetMod.get m1 MN1)).
       {
         assert (deadlocked m1 '' MN1) by eauto 4 using dep_self_deadlocked with LTS.
@@ -4953,11 +4953,11 @@ Module Type COMPL_F(Import Conf : DETECT_CONF)(Import Params : DETECT_PARAMS(Con
       + subst MN0'.
         smash_eq_on m0 m n; subst; hsimpl in *; hsimpl in |- *; eexists; eattac.
     - destruct S0 as [I0 P0 O0].
-      pose (NetMod.put n (mq MQ0 M1 (pq (I0 ++ [(m, &t, v)]) P0 O0)) MN0) as MN0'.
+      pose (NetMod.put n (mq MQ0 M1 (serv (I0 ++ [(m, &t, v)]) P0 O0)) MN0) as MN0'.
       exists (NTau n (MActP (Recv (m, &t) v))).
       exists MN0'.
       exists [].
-      exists (pq (I0 ++ [(m, &t, v)]) P0 O0).
+      exists (serv (I0 ++ [(m, &t, v)]) P0 O0).
       subst MN0' M1; attac.
       constructor. attac. constructor. rewrite H. attac.
       eexists. eattac.
@@ -5429,7 +5429,7 @@ Module Type COMPL_F(Import Conf : DETECT_CONF)(Import Params : DETECT_PARAMS(Con
       }
 
       destruct S1 as [I1 P1 O1].
-      pose (pq (I1 ++ [(m, Q, v)]) P1 O1) as S2.
+      pose (serv (I1 ++ [(m, Q, v)]) P1 O1) as S2.
       pose  {|self := self s
             ; lock_id := lock_id s
             ; lock := lock s
@@ -6438,7 +6438,7 @@ Module Type COMPL_F(Import Conf : DETECT_CONF)(Import Params : DETECT_PARAMS(Con
       }
 
       destruct S1 as [I1 P1 O1].
-      pose (pq (I1 ++ [(m, Q, v)]) P1 O1) as S2.
+      pose (serv (I1 ++ [(m, Q, v)]) P1 O1) as S2.
       pose  {|self := self s
             ; lock_id := lock_id s
             ; lock := lock s
@@ -6541,7 +6541,7 @@ Module Type COMPL_F(Import Conf : DETECT_CONF)(Import Params : DETECT_PARAMS(Con
   Qed.
 
   Lemma KIC_AnySRPC_pq_instr [I N] : KIC (net_instr I N) ->
-                                     forall n, AnySRPC_pq (NetMod.get n N).
+                                     forall n, AnySRPC_serv (NetMod.get n N).
   Proof.
     intros ?.
     consider (KIC _); attac.
